\section{Conclusioni}
[i cilindretti fanno cacare]



\begin{equation}
\tilde{D} = \frac{1}{N - 1} \sum_{i=1}^{N} (x_i - m^*[x])^2
\end{equation}

\begin{equation}
\tilde{\sigma} = \sqrt{\frac{1}{N - 1} \sum_{i=1}^{N} (x_i - m^*[x])^2}
\end{equation}

\begin{equation}
m^*[x] = \frac{1}{N} \sum_{i=1}^{N} (x_i) \simeq \sum_{j=1}^{\mathcal{N}} (x_j p_j^*) 
\end{equation}

\begin{equation}
p_j^* = \frac{n_j^*}{N} 
\end{equation}

\begin{equation}
f_j^* = \frac{n_j^*}{N\Delta x}
\end{equation}

\begin{equation}
D^* = \langle(x - m^*)^2\rangle = \frac{1}{N} \sum_{i=1}^{N} (x_i - m^*[x])^2
\simeq \sum_{j=1}^{\mathcal{N}} (x_j - m^*)^2 p_j^*)
\end{equation}

\begin{equation}
m^*[\mathcal{T}] = \frac{1}{N} \sum_{i=1}^{N} \mathcal{T}_i
\end{equation}

\begin{equation}
\sigma^*[\mathcal{T}] = \sqrt{\frac{1}{N} \sum_{i=1}^{N} (\mathcal{T}_i - m^*)^2}
\end{equation}

\begin{equation}
\mathcal{T} = \mathcal{T}_0 \pm \delta\mathcal{T}
\end{equation}

\begin{equation}
\mathcal{T}_0 = m^* = \frac{1}{N} \sum_{i=1}^{N} \mathcal{T}_i
\end{equation}

\begin{equation}
\delta\mathcal{T}_{cas} = \tilde{\sigma}[m^*] = \frac{1}{\sqrt{N}} \sqrt{\frac{N}{N - 1}}\sigma^*[\mathcal{T}] = \sqrt{\frac{1}{N(N - 1)} \sum_{i=1}^{N} (\mathcal{T}_i - m^*)^2}
\end{equation}

